finished EdmondsKarp correct and runtime proof

Examples/EdmondsKarp_Maxflow/EdmondsKarp_Algo.thy
@@ -14,52 +14,161 @@ subsection \<open>Algorithm\<close>
 context Network 
 begin
 
+
+definition "shortestpath_time = enat 10"
+                    
+lemma inresT_SELECT_Some: "inresT (SELECT Q tt) (Some x) t' \<longleftrightarrow> (Q x  \<and> (t' \<le> tt))"
+  by(auto simp: inresT_def SELECT_def emb'_def) 
+
+lemma inresT_SELECT_None: "inresT (SELECT Q tt) None t' \<longleftrightarrow> (\<not>(\<exists>x. Q x) \<and> (t' \<le> tt))"
+  by(auto simp: inresT_def SELECT_def emb'_def) 
+
+lemma inresT_SELECT[refine_pw_simps]:
+ "inresT (SELECT Q tt) x t' \<longleftrightarrow> ((case x of None \<Rightarrow> \<not>(\<exists>x. Q x) | Some x \<Rightarrow> Q x)  \<and> (t' \<le> tt))"
+  by(auto simp: inresT_def SELECT_def emb'_def) 
+
+
+lemma nofailT_SELECT[refine_pw_simps]: "nofailT (SELECT Q tt)"
+  by(auto simp: nofailT_def SELECT_def)
+
+lemma s1: "SELECT P T \<le> (SELECT P T') \<longleftrightarrow> T \<le> T'"
+  apply(cases "\<exists>x. P x") 
+   apply(auto simp: pw_le_iff refine_pw_simps split: option.splits)
+  subgoal 
+    by (metis (full_types) enat_ord_code(3) enat_ord_simps(1) lessI not_infinity_eq not_le order_mono_setup.refl) 
+  subgoal 
+    by (metis (full_types) enat_ord_code(3) enat_ord_simps(1) lessI not_enat_eq not_le order_mono_setup.refl) 
+  done
+     
+lemma s2: "SELECT P T \<le> (SELECT P' T) \<longleftrightarrow> (
+    (Ex P' \<longrightarrow> Ex P)  \<and> (\<forall>x. P x \<longrightarrow> P' x)) "
+  apply(auto simp: pw_le_iff refine_pw_simps split: option.splits)
+  subgoal 
+    by (metis enat_ile linear)                                          
+  subgoal 
+    by (metis enat_ile linear) 
+  done
+ 
+lemma SELECT_refine:
+  assumes "\<And>x'. P' x' \<Longrightarrow> \<exists>x. P x"
+  assumes "\<And>x. P x \<Longrightarrow>   P' x"
+  assumes "T \<le> T'"
+  shows "SELECT P T \<le> (SELECT P' T')"
+proof -
+  have "SELECT P T \<le> SELECT P T'"
+    using s1 assms(3) by auto
+  also have "\<dots> \<le> SELECT P' T'"
+    unfolding s2 apply safe
+    using assms(1,2) by auto  
+  finally show ?thesis .
+qed
+ 
+
+
 text \<open>First, we specify the refined procedure for finding augmenting paths\<close>
-definition "find_shortest_augmenting_spec f \<equiv> assert (NFlow c s t f) \<then> 
-  (select p. Graph.isShortestPath (residualGraph c f) s p t)"
+definition "find_shortest_augmenting_spec f \<equiv> ASSERT (NFlow c s t f) \<then> 
+  SELECT (\<lambda>p. Graph.isShortestPath (residualGraph c f) s p t) (shortestpath_time)"
 
 text \<open>We show that our refined procedure is actually a refinement\<close>  
-thm SELECT_refine  
-lemma find_shortest_augmenting_refine[refine]: 
+lemma find_shortest_augmenting_refine: 
   "(f',f)\<in>Id \<Longrightarrow> find_shortest_augmenting_spec f' \<le> \<Down>(\<langle>Id\<rangle>option_rel) (find_augmenting_spec f)"  
   unfolding find_shortest_augmenting_spec_def find_augmenting_spec_def
-  apply (refine_vcg)
-  apply (auto 
-    simp: NFlow.shortest_is_augmenting RELATESI
-    dest: NFlow.augmenting_path_imp_shortest)
-  done
+  apply(rule bindT_refine'[where R'=Id])
+   apply auto 
+  apply(rule SELECT_refine)
+  subgoal unfolding special_info_def by auto
+  subgoal unfolding special_info_def apply safe
+    using NFlow.shortest_is_augmenting  
+      NFlow.augmenting_path_imp_shortest pw_ASSERT 
+    by blast 
+  unfolding shortestpath_time_def find_augmenting_time_def by simp
 
 text \<open>Next, we specify the Edmonds-Karp algorithm. 
   Our first specification still uses partial correctness, 
   termination will be proved afterwards. \<close>  
 definition "edka_partial \<equiv> do {
-  let f = (\<lambda>_. 0);
+  f \<leftarrow> RETURNT (\<lambda>_. 0);
 
-  (f,_) \<leftarrow> while\<^bsup>fofu_invar\<^esup>
+  (f,_) \<leftarrow> whileT(*\<^bsup>fofu_invar\<^esup>*)
     (\<lambda>(f,brk). \<not>brk) 
     (\<lambda>(f,_). do {
       p \<leftarrow> find_shortest_augmenting_spec f;
       case p of 
-        None \<Rightarrow> return (f,True)
+        None \<Rightarrow> RETURNT (f,True)
       | Some p \<Rightarrow> do {
-          assert (p\<noteq>[]);
-          assert (NPreflow.isAugmentingPath c s t f p);
-          assert (Graph.isShortestPath (residualGraph c f) s p t);
-          let f = NFlow.augment_with_path c f p;
-          assert (NFlow c s t f);
-          return (f, False)
+          ASSERT (p\<noteq>[]);
+          ASSERT (NPreflow.isAugmentingPath c s t f p);
+          ASSERT (Graph.isShortestPath (residualGraph c f) s p t);
+          f \<leftarrow> RETURNT (NFlow.augment_with_path c f p);
+          ASSERT (NFlow c s t f);
+          RETURNT (f, False)
         }  
     })
     (f,False);
-  assert (NFlow c s t f);
-  return f 
-}"
+  ASSERT (NFlow c s t f);
+  RETURNT f 
+}" 
+ 
 
-lemma edka_partial_refine[refine]: "edka_partial \<le> \<Down>Id fofu"
-  unfolding edka_partial_def fofu_def
-  apply (refine_rcg bind_refine')
-  apply (refine_dref_type)
-  apply (vc_solve simp: find_shortest_augmenting_spec_def)
+lemma case_prod_refine:
+  fixes P Q :: "'a \<Rightarrow> 'b \<Rightarrow> 'c nrest"
+  assumes
+    "\<And>a b. P a b \<le> Q a b"
+  shows
+ "(case x of (a,b) \<Rightarrow> P a b) \<le> (case x of (a,b) \<Rightarrow> Q a b)"
+  using assms 
+  by (simp add: split_def)
+
+lemma case_option_refine:
+  fixes P Q :: "'a \<Rightarrow> 'b \<Rightarrow> 'c nrest"
+  assumes
+    "PN \<le> QN"
+    "\<And>a. PS a \<le> QS a"
+  shows
+ "(case x of None \<Rightarrow> PN | Some a \<Rightarrow> PS a ) \<le> (case x of None \<Rightarrow> QN | Some a \<Rightarrow> QS a )"
+  using assms 
+  by (auto split: option.splits)
+
+lemma ASSERT_refine: "(Q \<Longrightarrow> P) \<Longrightarrow> ASSERT P \<le> ASSERT Q"
+  by(auto simp: pw_le_iff refine_pw_simps)
+
+lemma ASSERT_leI: "\<Phi> \<Longrightarrow> (\<Phi> \<Longrightarrow> M \<le> M') \<Longrightarrow> ASSERT \<Phi> \<bind> (\<lambda>_. M) \<le> M'"
+  by(auto simp: pw_le_iff refine_pw_simps)
+lemma le_ASSERTI: "(\<Phi> \<Longrightarrow> M \<le> M') \<Longrightarrow> M \<le> ASSERT \<Phi> \<bind> (\<lambda>_. M')"
+  by(auto simp: pw_le_iff refine_pw_simps)
+
+thm refine_mono
+
+lemma inresT_ASSERT: "inresT (ASSERT Q \<bind> (\<lambda>_. M)) x ta = (Q \<longrightarrow> inresT M x ta)"
+  unfolding ASSERT_def iASSERT_def by auto
+
+
+lemma nofailT_ASSERT_bind: "nofailT (ASSERT P \<bind> (\<lambda>_. M)) \<longleftrightarrow> (P \<and> nofailT M)"
+  by(auto simp: pw_bindT_nofailT pw_ASSERT)
+
+
+lemma edka_partial_refine : "edka_partial \<le> \<Down>Id fofu"
+  unfolding edka_partial_def fofu_def 
+  apply(rule bindT_refine'[where R'=Id])
+  apply simp
+  apply(rule bindT_refine'[where R'="Id"])
+   apply simp
+   apply(rule whileT_mono)
+   apply(rule case_prod_refine)
+   apply auto   
+  apply(rule bindT_mono) apply auto
+  subgoal 
+    using find_shortest_augmenting_refine[simplified option_rel_id_simp, simplified] by simp
+  subgoal 
+    apply(rule case_option_mono) apply simp  
+    apply(rule le_ASSERTI)+   
+    apply(rule ASSERT_leI | simp)+
+    unfolding find_shortest_augmenting_spec_def
+    subgoal apply(simp only: inresT_ASSERT inresT_SELECT_Some)  apply safe
+      unfolding find_augmenting_spec_def (* WHY DO I NEED TO RECOVER ALL THIS INFORMATION FROM THE
+          inresT and nofailT predicate?! *)      
+      by(simp add: nofailT_ASSERT_bind)
+    by(rule ASSERT_leI | simp)+     
   done
 
 
@@ -69,26 +178,26 @@ subsubsection \<open>Total Correctness\<close>
 context Network begin
 text \<open>We specify the total correct version of Edmonds-Karp algorithm.\<close>
 definition "edka \<equiv> do {
-  let f = (\<lambda>_. 0);
+  f \<leftarrow> RETURNT (\<lambda>_. 0);
 
-  (f,_) \<leftarrow> while\<^sub>T\<^bsup>fofu_invar\<^esup>
+  (f,_) \<leftarrow> whileT(*\<^bsup>fofu_invar\<^esup>*)
     (\<lambda>(f,brk). \<not>brk) 
     (\<lambda>(f,_). do {
       p \<leftarrow> find_shortest_augmenting_spec f;
       case p of 
-        None \<Rightarrow> return (f,True)
+        None \<Rightarrow> RETURNT (f,True)
       | Some p \<Rightarrow> do {
-          assert (p\<noteq>[]);
-          assert (NPreflow.isAugmentingPath c s t f p);
-          assert (Graph.isShortestPath (residualGraph c f) s p t);
-          let f = NFlow.augment_with_path c f p;
-          assert (NFlow c s t f);
-          return (f, False)
+          ASSERT (p\<noteq>[]);
+          ASSERT (NPreflow.isAugmentingPath c s t f p);
+          ASSERT (Graph.isShortestPath (residualGraph c f) s p t);
+          f \<leftarrow> RETURNT (NFlow.augment_with_path c f p);
+          ASSERT (NFlow c s t f);
+          RETURNT (f, False)
         }  
     })
     (f,False);
-  assert (NFlow c s t f);
-  return f 
+  ASSERT (NFlow c s t f);
+  RETURNT f 
 }"
 
 text \<open>Based on the measure function, it is easy to obtain a well-founded 
@@ -102,28 +211,17 @@ lemma edka_wf_rel_wf[simp, intro!]: "wf edka_wf_rel"
 
 text \<open>The following theorem states that the total correct 
   version of Edmonds-Karp algorithm refines the partial correct one.\<close>  
-theorem edka_refine[refine]: "edka \<le> \<Down>Id edka_partial"
+theorem edka_refine: "edka \<le> \<Down>Id edka_partial"
   unfolding edka_def edka_partial_def
-  apply (refine_rcg bind_refine' 
-    WHILEIT_refine_WHILEI[where V=edka_wf_rel])
-  apply (refine_dref_type)
-  apply (simp; fail)
-  subgoal
-    txt \<open>Unfortunately, the verification condition for introducing 
-      the variant requires a bit of manual massaging to be solved:\<close>
-    apply (simp)
-    apply (erule bind_sim_select_rule)
-    apply (auto split: option.split 
-      simp: NFlow.augment_with_path_def
-      simp: assert_bind_spec_conv Let_def
-      simp: find_shortest_augmenting_spec_def
-      simp: edka_wf_rel_def NFlow.shortest_path_decr_ek_measure
-    ; fail) []
-  done
+  by simp 
+ 
 
-  txt \<open>The other VCs are straightforward\<close>
-  apply (vc_solve)
-  done
+thm edka_refine edka_partial_refine fofu_partial_correct
+
+lemma edka_correct_time: "edka \<le> SPECT (emb isMaxFlow maxFlow_time)" 
+  using edka_refine edka_partial_refine fofu_partial_correct 
+  by simp
+
 
 subsubsection \<open>Complexity Analysis\<close>
 
@@ -187,58 +285,22 @@ text \<open>Finally, we present a version of the Edmonds-Karp algorithm
   Note that we only count the non-breaking loop iterations.
   \<close>
 
-text \<open>The refinement is achieved by a refinement relation, coupling the 
-  instrumented loop state with the uninstrumented one\<close>
-definition "edkac_rel \<equiv> {((f,brk,itc), (f,brk)) | f brk itc.
-    itc + ek_analysis_defs.ekMeasure (residualGraph c f) s t 
-  < 2 * card V * card E + card V
-}"
 
-definition "edka_complexity \<equiv> do {
-  let f = (\<lambda>_. 0);
+lemma maxFlow_time_ub: "maxFlow_time \<le> find_augmenting_time (\<lambda>_. 0) * ((2 * card V * card E + card V) + 1)"
+  unfolding maxFlow_time_def R_def 
+  using ekMeasure_upper_bound 
+  by (meson enat_ord_simps(2) le_iff_add less_le less_le_trans linorder_not_le nat_mult_less_cancel_disj)
 
-  (f,_,itc) \<leftarrow> while\<^sub>T 
-    (\<lambda>(f,brk,_). \<not>brk) 
-    (\<lambda>(f,_,itc). do {
-      p \<leftarrow> find_shortest_augmenting_spec f;
-      case p of 
-        None \<Rightarrow> return (f,True,itc)
-      | Some p \<Rightarrow> do {
-          let f = NFlow.augment_with_path c f p;
-          return (f, False,itc + 1)
-        }  
-    })
-    (f,False,0);
-  assert (itc < 2 * card V * card E + card V);
-  return f 
-}"
-  
-lemma edka_complexity_refine: "edka_complexity \<le> \<Down>Id edka"
-proof -
-  have [refine_dref_RELATES]: 
-    "RELATES edkac_rel"
-    by (auto simp: RELATES_def)
 
-  show ?thesis  
-    unfolding edka_complexity_def edka_def
-    apply (refine_rcg)
-    apply (refine_dref_type)
-    apply (vc_solve simp: edkac_rel_def "NFlow.augment_with_path_def")
-    subgoal using ekMeasure_upper_bound by auto []
-    subgoal by (drule (1) NFlow.shortest_path_decr_ek_measure; auto)
-    done
-qed    
+lemma SPECT_ub: "T\<le>T' \<Longrightarrow> SPECT (emb' M' T) \<le> SPECT (emb' M' T')"
+  unfolding emb'_def by (auto simp: pw_le_iff le_funD order_trans refine_pw_simps)
 
-text \<open>We show that this algorithm never fails, and computes a maximum flow.\<close>
-theorem "edka_complexity \<le> (spec f. isMaxFlow f)"
-proof -  
-  note edka_complexity_refine
-  also note edka_refine
-  also note edka_partial_refine
-  also note fofu_partial_correct
-  finally show ?thesis .
-qed  
-
+lemma "edka \<le> (SPECT (emb isMaxFlow (find_augmenting_time (\<lambda>_. 0) * ((2 * card V * card E + card V) + 1))))"
+  apply(rule order_trans[OF edka_correct_time]) 
+  apply(rule SPECT_ub)
+  apply (simp only: le_fun_def)
+    using  maxFlow_time_ub by simp  
+ 
 
 end \<comment> \<open>Network\<close>
 end \<comment> \<open>Theory\<close>
